new/golang/theory/intoval.v
@@ -1,5 +1,4 @@
 From Coq Require Import Logic.FunctionalExtensionality.
-From Coq Require Import Program.Equality.
 From iris.bi.lib Require Import fractional.
 From Perennial.goose_lang Require Export lang lifting ipersist.
 From stdpp Require Import list.
@@ -13,9 +12,9 @@ Context `{sem: ffi_semantics} `{!ffi_interp ffi} `{!heapGS Σ} `{!GoContext}.
 
 Class IntoValComparable (V : Type) `{!IntoVal V} :=
   {
-    #[global] to_val_inj :: Inj (=) (=) (to_val (V:=V));
-    #[global] to_val_eqdec :: EqDecision V ;
-    to_val_comparable : (∀ (v : V), is_comparable #v);
+    #[global] into_val_inj :: Inj (=) (=) (into_val (V:=V));
+    #[global] into_val_eqdec :: EqDecision V ;
+    into_val_comparable : (∀ (v : V), is_comparable #v);
   }.
 
 Class TypedPointsto (V : Type) `{!IntoVal V} :=
@@ -62,3 +61,76 @@ Global Arguments wp_store {_ _ _ _ _ _ _} [_ _ _ _ _] (l v w Φ).
 Notation "l ↦ dq v" := (typed_pointsto l dq v%V)
                          (at level 20, dq custom dfrac at level 1,
                             format "l  ↦ dq  v") : bi_scope.
+
+Set Default Proof Using "Type".
+
+Section into_val_instances.
+Context `{sem: ffi_semantics} `{!ffi_interp ffi} `{!heapGS Σ} {Hvalid : go.ValidCore}.
+
+(** TypedPointsto instances *)
+Program Global Instance typed_pointsto_loc : TypedPointsto loc :=
+  {| typed_pointsto_def l dq v := heap_pointsto l dq #v |}.
+
+Program Global Instance typed_pointsto_w64 : TypedPointsto w64 :=
+  {| typed_pointsto_def l dq v := heap_pointsto l dq #v |}.
+
+Program Global Instance typed_pointsto_w32 : TypedPointsto w32 :=
+  {| typed_pointsto_def l dq v := heap_pointsto l dq #v |}.
+
+Program Global Instance typed_pointsto_w16 : TypedPointsto w16 :=
+  {| typed_pointsto_def l dq v := heap_pointsto l dq #v |}.
+
+Program Global Instance typed_pointsto_w8 : TypedPointsto w8 :=
+  {| typed_pointsto_def l dq v := heap_pointsto l dq #v |}.
+
+Program Global Instance typed_pointsto_bool : TypedPointsto bool :=
+  {| typed_pointsto_def l dq v := heap_pointsto l dq #v |}.
+
+Program Global Instance typed_pointsto_string : TypedPointsto go_string :=
+  {| typed_pointsto_def l dq v := heap_pointsto l dq #v |}.
+
+Program Global Instance typed_pointsto_slice : TypedPointsto slice.t :=
+  {| typed_pointsto_def l dq v := heap_pointsto l dq #v |}.
+
+Program Global Instance typed_pointsto_func : TypedPointsto func.t :=
+  {| typed_pointsto_def l dq v := heap_pointsto l dq #v |}.
+
+Program Global Instance typed_pointsto_array (V : Type) `{!IntoVal V} n
+  `{!TypedPointsto V} `{!IntoValTyped V t} : TypedPointsto (array.t t V n) :=
+  {|
+    typed_pointsto_def l dq v :=
+      ([∗ list] i ↦ ve ∈ (vec_to_list v.(array.vec)), array_index_ref t (Z.of_nat i) l ↦ ve)%I;
+  |}.
+
+(** IntoValComparable instances *)
+Ltac solve_into_val_comparable :=
+  split;
+  [rewrite into_val_unseal; intros ??; by inversion 1|
+    apply _ |
+    rewrite into_val_unseal; done].
+
+Global Instance into_val_comparable_loc : IntoValComparable loc.
+Proof. solve_into_val_comparable. Qed.
+
+Global Instance into_val_comparable_w64 : IntoValComparable w64.
+Proof. solve_into_val_comparable. Qed.
+
+Global Instance into_val_comparable_w32 : IntoValComparable w32.
+Proof. solve_into_val_comparable. Qed.
+
+Global Instance into_val_comparable_w16 : IntoValComparable w16.
+Proof. solve_into_val_comparable. Qed.
+
+Global Instance into_val_comparable_w8 : IntoValComparable w8.
+Proof. solve_into_val_comparable. Qed.
+
+Global Instance into_val_comparable_bool : IntoValComparable bool.
+Proof. solve_into_val_comparable. Qed.
+
+Global Instance into_val_comparable_string : IntoValComparable go_string.
+Proof. solve_into_val_comparable. Qed.
+
+Global Instance into_val_comparable_slice : IntoValComparable slice.t.
+Proof. solve_into_val_comparable. Qed.
+
+End into_val_instances.
