new/golang/theory/proofmode.v
@@ -88,16 +88,16 @@ Global Instance wp_fst (v1 v2 : val) : PureWp True (Fst (v1, v2)%V) v1.
 Proof. apply (pure_exec_pure_wp O). solve_pure_exec. Qed.
 
 Global Instance wp_recc f x erec : PureWp True (rec: f x := erec)%E #(func.mk f x erec).
-Proof. rewrite to_val_unseal. apply (pure_exec_pure_wp O). solve_pure_exec. Qed.
+Proof. rewrite into_val_unseal. apply (pure_exec_pure_wp O). solve_pure_exec. Qed.
 
 Global Instance wp_pair (v1 v2 : val) : PureWp True (v1, v2)%E (v1, v2)%V.
 Proof. apply (pure_exec_pure_wp O). solve_pure_exec. Qed.
 
 Global Instance wp_if_false e1 e2 : PureWp True (if: #false then e1 else e2) e2.
-Proof. apply (pure_exec_pure_wp O). rewrite to_val_unseal. solve_pure_exec. Qed.
+Proof. apply (pure_exec_pure_wp O). rewrite into_val_unseal. solve_pure_exec. Qed.
 
 Global Instance wp_if_true e1 e2 : PureWp True (if: #true then e1 else e2) e1.
-Proof. apply (pure_exec_pure_wp O). rewrite to_val_unseal. solve_pure_exec. Qed.
+Proof. apply (pure_exec_pure_wp O). rewrite into_val_unseal. solve_pure_exec. Qed.
 
 Global Instance wp_case_inr v e1 e2 : PureWp True (Case (InjRV v) e1 e2) (e2 v).
 Proof. apply (pure_exec_pure_wp O). solve_pure_exec. Qed.
@@ -111,7 +111,7 @@ Proof.
   apply (pure_exec_pure_wp O).
   intros Hcomp.
   cut (bin_op_eval EqOp v1 v2 = Some $ LitV $ LitBool $ bool_decide (v1 = v2)).
-  { rewrite to_val_unseal. solve_pure_exec. }
+  { rewrite into_val_unseal. solve_pure_exec. }
   rewrite /bin_op_eval /bin_op_eval_eq /=.
   rewrite decide_True //.
 Qed.
@@ -119,152 +119,152 @@ Qed.
 (** Unops *)
 (* w64 unops *)
 Global Instance wp_neg_w64 (v : w64) : PureWp True (~#v) #(word.not v).
-Proof. rewrite to_val_unseal. apply (pure_exec_pure_wp O). solve_pure_exec. Qed.
+Proof. rewrite into_val_unseal. apply (pure_exec_pure_wp O). solve_pure_exec. Qed.
 
 Global Instance wp_w64_u_to_w64 (v : w64) : PureWp True (u_to_w64 #v) #v.
 Proof.
-  rewrite to_val_unseal. apply (pure_exec_pure_wp O).
+  rewrite into_val_unseal. apply (pure_exec_pure_wp O).
   solve_pure_exec. replace (_ (uint.Z v)) with v by word. done.
 Qed.
 
 Global Instance wp_w64_u_to_w32 (v : w64) : PureWp True (u_to_w32 #v) #(W32 $ uint.Z v).
-Proof. rewrite to_val_unseal. apply (pure_exec_pure_wp O). solve_pure_exec. Qed.
+Proof. rewrite into_val_unseal. apply (pure_exec_pure_wp O). solve_pure_exec. Qed.
 
 Global Instance wp_w64_u_to_w16 (v : w64) : PureWp True (u_to_w16 #v) #(W16 $ uint.Z v).
-Proof. rewrite to_val_unseal. apply (pure_exec_pure_wp O). solve_pure_exec. Qed.
+Proof. rewrite into_val_unseal. apply (pure_exec_pure_wp O). solve_pure_exec. Qed.
 
 Global Instance wp_w64_u_to_w8 (v : w64) : PureWp True (u_to_w8 #v) #(W8 $ uint.Z v).
-Proof. rewrite to_val_unseal. apply (pure_exec_pure_wp O). solve_pure_exec. Qed.
+Proof. rewrite into_val_unseal. apply (pure_exec_pure_wp O). solve_pure_exec. Qed.
 
 Global Instance wp_w64_s_to_w64 (v : w64) : PureWp True (s_to_w64 #v) #v.
 Proof.
-  rewrite to_val_unseal. apply (pure_exec_pure_wp O).
+  rewrite into_val_unseal. apply (pure_exec_pure_wp O).
   solve_pure_exec. replace (_ (sint.Z v)) with v by word. done.
 Qed.
 
 Global Instance wp_w64_s_to_w32 (v : w64) : PureWp True (s_to_w32 #v) #(W32 $ sint.Z v).
-Proof. rewrite to_val_unseal. apply (pure_exec_pure_wp O). solve_pure_exec. Qed.
+Proof. rewrite into_val_unseal. apply (pure_exec_pure_wp O). solve_pure_exec. Qed.
 
 Global Instance wp_w64_s_to_w16 (v : w64) : PureWp True (s_to_w16 #v) #(W16 $ sint.Z v).
-Proof. rewrite to_val_unseal. apply (pure_exec_pure_wp O). solve_pure_exec. Qed.
+Proof. rewrite into_val_unseal. apply (pure_exec_pure_wp O). solve_pure_exec. Qed.
 
 Global Instance wp_w64_s_to_w8 (v : w64) : PureWp True (s_to_w8 #v) #(W8 $ sint.Z v).
-Proof. rewrite to_val_unseal. apply (pure_exec_pure_wp O). solve_pure_exec. Qed.
+Proof. rewrite into_val_unseal. apply (pure_exec_pure_wp O). solve_pure_exec. Qed.
 
 (* w32 unops *)
 Global Instance wp_neg_w32 (v : w32) : PureWp True (~#v) #(word.not v).
-Proof. rewrite to_val_unseal. apply (pure_exec_pure_wp O). solve_pure_exec. Qed.
+Proof. rewrite into_val_unseal. apply (pure_exec_pure_wp O). solve_pure_exec. Qed.
 
 Global Instance wp_w32_u_to_w64 (v : w32) : PureWp True (u_to_w64 #v) #(W64 $ uint.Z v).
-Proof. rewrite to_val_unseal. apply (pure_exec_pure_wp O). solve_pure_exec. Qed.
+Proof. rewrite into_val_unseal. apply (pure_exec_pure_wp O). solve_pure_exec. Qed.
 
 Global Instance wp_w32_u_to_w32 (v : w32) : PureWp True (u_to_w32 #v) #v.
 Proof.
-  rewrite to_val_unseal. apply (pure_exec_pure_wp O).
+  rewrite into_val_unseal. apply (pure_exec_pure_wp O).
   solve_pure_exec. replace (_ (uint.Z v)) with v by word. done.
 Qed.
 
 Global Instance wp_w32_u_to_w16 (v : w32) : PureWp True (u_to_w16 #v) #(W16 $ uint.Z v).
-Proof. rewrite to_val_unseal. apply (pure_exec_pure_wp O). solve_pure_exec. Qed.
+Proof. rewrite into_val_unseal. apply (pure_exec_pure_wp O). solve_pure_exec. Qed.
 
 Global Instance wp_w32_u_to_w8 (v : w32) : PureWp True (u_to_w8 #v) #(W8 $ uint.Z v).
-Proof. rewrite to_val_unseal. apply (pure_exec_pure_wp O). solve_pure_exec. Qed.
+Proof. rewrite into_val_unseal. apply (pure_exec_pure_wp O). solve_pure_exec. Qed.
 
 Global Instance wp_w32_s_to_w64 (v : w32) : PureWp True (s_to_w64 #v) #(W64 $ sint.Z v).
-Proof. rewrite to_val_unseal. apply (pure_exec_pure_wp O). solve_pure_exec. Qed.
+Proof. rewrite into_val_unseal. apply (pure_exec_pure_wp O). solve_pure_exec. Qed.
 
 Global Instance wp_w32_s_to_w32 (v : w32) : PureWp True (s_to_w32 #v) #v.
 Proof.
-  rewrite to_val_unseal. apply (pure_exec_pure_wp O).
+  rewrite into_val_unseal. apply (pure_exec_pure_wp O).
   solve_pure_exec. replace (_ (sint.Z v)) with v by word. done.
 Qed.
 
 Global Instance wp_w32_s_to_w16 (v : w32) : PureWp True (s_to_w16 #v) #(W16 $ sint.Z v).
-Proof. rewrite to_val_unseal. apply (pure_exec_pure_wp O). solve_pure_exec. Qed.
+Proof. rewrite into_val_unseal. apply (pure_exec_pure_wp O). solve_pure_exec. Qed.
 
 Global Instance wp_w32_s_to_w8 (v : w32) : PureWp True (s_to_w8 #v) #(W8 $ sint.Z v).
-Proof. rewrite to_val_unseal. apply (pure_exec_pure_wp O). solve_pure_exec. Qed.
+Proof. rewrite into_val_unseal. apply (pure_exec_pure_wp O). solve_pure_exec. Qed.
 
 (* w8 unops *)
 Global Instance wp_neg_w8 (v : w8) : PureWp True (~#v) #(word.not v).
-Proof. rewrite to_val_unseal. apply (pure_exec_pure_wp O). solve_pure_exec. Qed.
+Proof. rewrite into_val_unseal. apply (pure_exec_pure_wp O). solve_pure_exec. Qed.
 
 Global Instance wp_w8_u_to_w64 (v : w8) : PureWp True (u_to_w64 #v) #(W64 $ uint.Z v).
-Proof. rewrite to_val_unseal. apply (pure_exec_pure_wp O). solve_pure_exec. Qed.
+Proof. rewrite into_val_unseal. apply (pure_exec_pure_wp O). solve_pure_exec. Qed.
 
 Global Instance wp_w8_u_to_w32 (v : w8) : PureWp True (u_to_w32 #v) #(W32 $ uint.Z v).
-Proof. rewrite to_val_unseal. apply (pure_exec_pure_wp O). solve_pure_exec. Qed.
+Proof. rewrite into_val_unseal. apply (pure_exec_pure_wp O). solve_pure_exec. Qed.
 
 Global Instance wp_w8_u_to_w8 (v : w8) : PureWp True (u_to_w8 #v) #v.
 Proof.
-  rewrite to_val_unseal. apply (pure_exec_pure_wp O).
+  rewrite into_val_unseal. apply (pure_exec_pure_wp O).
   solve_pure_exec. replace (_ (uint.Z v)) with v by word. done.
 Qed.
 
 Global Instance wp_w8_s_to_w64 (v : w8) : PureWp True (s_to_w64 #v) #(W64 $ sint.Z v).
-Proof. rewrite to_val_unseal. apply (pure_exec_pure_wp O). solve_pure_exec. Qed.
+Proof. rewrite into_val_unseal. apply (pure_exec_pure_wp O). solve_pure_exec. Qed.
 
 Global Instance wp_w8_s_to_w32 (v : w8) : PureWp True (s_to_w32 #v) #(W32 $ sint.Z v).
-Proof. rewrite to_val_unseal. apply (pure_exec_pure_wp O). solve_pure_exec. Qed.
+Proof. rewrite into_val_unseal. apply (pure_exec_pure_wp O). solve_pure_exec. Qed.
 
 Global Instance wp_w8_s_to_w8 (v : w8) : PureWp True (s_to_w8 #v) #v.
 Proof.
-  rewrite to_val_unseal. apply (pure_exec_pure_wp O).
+  rewrite into_val_unseal. apply (pure_exec_pure_wp O).
   solve_pure_exec. replace (_ (sint.Z v)) with v by word. done.
 Qed.
 
 Global Instance wp_w8_to_string (v : w8) : PureWp True (to_string #v) #([v]).
-Proof. rewrite to_val_unseal. apply (pure_exec_pure_wp O). solve_pure_exec. Qed.
+Proof. rewrite into_val_unseal. apply (pure_exec_pure_wp O). solve_pure_exec. Qed.
 
 (* w16 unops *)
 Global Instance wp_neg_w16 (v : w16) : PureWp True (~#v) #(word.not v).
-Proof. rewrite to_val_unseal. apply (pure_exec_pure_wp O). solve_pure_exec. Qed.
+Proof. rewrite into_val_unseal. apply (pure_exec_pure_wp O). solve_pure_exec. Qed.
 
 Global Instance wp_w16_u_to_w64 (v : w16) : PureWp True (u_to_w64 #v) #(W64 $ uint.Z v).
-Proof. rewrite to_val_unseal. apply (pure_exec_pure_wp O). solve_pure_exec. Qed.
+Proof. rewrite into_val_unseal. apply (pure_exec_pure_wp O). solve_pure_exec. Qed.
 
 Global Instance wp_w16_u_to_w32 (v : w16) : PureWp True (u_to_w32 #v) #(W32 $ uint.Z v).
-Proof. rewrite to_val_unseal. apply (pure_exec_pure_wp O). solve_pure_exec. Qed.
+Proof. rewrite into_val_unseal. apply (pure_exec_pure_wp O). solve_pure_exec. Qed.
 
 Global Instance wp_w16_u_to_w16 (v : w16) : PureWp True (u_to_w16 #v) #(W16 $ uint.Z v).
-Proof. rewrite to_val_unseal. apply (pure_exec_pure_wp O). solve_pure_exec. Qed.
+Proof. rewrite into_val_unseal. apply (pure_exec_pure_wp O). solve_pure_exec. Qed.
 
 Global Instance wp_w16_u_to_w8 (v : w16) : PureWp True (u_to_w8 #v) #(W8 $ uint.Z v).
-Proof. rewrite to_val_unseal. apply (pure_exec_pure_wp O). solve_pure_exec. Qed.
+Proof. rewrite into_val_unseal. apply (pure_exec_pure_wp O). solve_pure_exec. Qed.
 
 Global Instance wp_w16_s_to_w64 (v : w16) : PureWp True (s_to_w64 #v) #(W64 $ sint.Z v).
-Proof. rewrite to_val_unseal. apply (pure_exec_pure_wp O). solve_pure_exec. Qed.
+Proof. rewrite into_val_unseal. apply (pure_exec_pure_wp O). solve_pure_exec. Qed.
 
 Global Instance wp_w16_s_to_w32 (v : w16) : PureWp True (s_to_w32 #v) #(W32 $ sint.Z v).
-Proof. rewrite to_val_unseal. apply (pure_exec_pure_wp O). solve_pure_exec. Qed.
+Proof. rewrite into_val_unseal. apply (pure_exec_pure_wp O). solve_pure_exec. Qed.
 
 Global Instance wp_w16_s_to_w16 (v : w16) : PureWp True (s_to_w16 #v) #(W16 $ sint.Z v).
-Proof. rewrite to_val_unseal. apply (pure_exec_pure_wp O). solve_pure_exec. Qed.
+Proof. rewrite into_val_unseal. apply (pure_exec_pure_wp O). solve_pure_exec. Qed.
 
 Global Instance wp_w16_s_to_w8 (v : w16) : PureWp True (s_to_w8 #v) #(W8 $ sint.Z v).
-Proof. rewrite to_val_unseal. apply (pure_exec_pure_wp O). solve_pure_exec. Qed.
+Proof. rewrite into_val_unseal. apply (pure_exec_pure_wp O). solve_pure_exec. Qed.
 
 (* bool unop *)
 Global Instance wp_bool_neg (b : bool) : PureWp True (~ #b) #(negb b).
-Proof. rewrite to_val_unseal. apply (pure_exec_pure_wp O). solve_pure_exec. Qed.
+Proof. rewrite into_val_unseal. apply (pure_exec_pure_wp O). solve_pure_exec. Qed.
 
 (* string unop *)
 Global Instance wp_StringLength (s : go_string) : PureWp True (StringLength #s) #(W64 $ length s).
-Proof. rewrite to_val_unseal. apply (pure_exec_pure_wp O). solve_pure_exec. Qed.
+Proof. rewrite into_val_unseal. apply (pure_exec_pure_wp O). solve_pure_exec. Qed.
 
 Global Instance wp_IsNoStringOverflow (s : go_string) : PureWp True (IsNoStringOverflow #s)
                                                        #(bool_decide ((length s) < 2^64)).
-Proof. rewrite to_val_unseal. apply (pure_exec_pure_wp O). solve_pure_exec. Qed.
+Proof. rewrite into_val_unseal. apply (pure_exec_pure_wp O). solve_pure_exec. Qed.
 
 (** Binops *)
 
 (* w64 binop instance *)
 Global Instance wp_w64_binop op (v1 v2 : w64) (v : val) :
   PureWp (op ≠ EqOp ∧
-      (to_val <$> bin_op_eval_word op v1 v2) ∪ (to_val <$> bin_op_eval_compare op v1 v2) = Some v)
+      (into_val <$> bin_op_eval_word op v1 v2) ∪ (into_val <$> bin_op_eval_compare op v1 v2) = Some v)
     (BinOp op #v1 #v2)%E v | 1.
 Proof.
-  rewrite to_val_unseal /=. apply (pure_exec_pure_wp O).
+  rewrite into_val_unseal /=. apply (pure_exec_pure_wp O).
   intros [??]. assert (bin_op_eval op (LitV v1) (LitV v2) = Some v).
   { rewrite /bin_op_eval decide_False // /=. destruct op; try by simpl in *. }
   revert H. solve_pure_exec.
@@ -272,10 +272,10 @@ Qed.
 
 Global Instance wp_w32_binop op (v1 v2 : w32) (v : val) :
   PureWp (op ≠ EqOp ∧
-      (to_val <$> bin_op_eval_word op v1 v2) ∪ (to_val <$> bin_op_eval_compare op v1 v2) = Some v)
+      (into_val <$> bin_op_eval_word op v1 v2) ∪ (into_val <$> bin_op_eval_compare op v1 v2) = Some v)
     (BinOp op #v1 #v2)%E v | 1.
 Proof.
-  rewrite to_val_unseal /=. apply (pure_exec_pure_wp O).
+  rewrite into_val_unseal /=. apply (pure_exec_pure_wp O).
   intros [??]. assert (bin_op_eval op (LitV v1) (LitV v2) = Some v).
   { rewrite /bin_op_eval decide_False // /=. destruct op; try by simpl in *. }
   revert H. solve_pure_exec.
@@ -283,10 +283,10 @@ Qed.
 
 Global Instance wp_w16_binop op (v1 v2 : w16) (v : val) :
   PureWp (op ≠ EqOp ∧
-      (to_val <$> bin_op_eval_word op v1 v2) ∪ (to_val <$> bin_op_eval_compare op v1 v2) = Some v)
+      (into_val <$> bin_op_eval_word op v1 v2) ∪ (into_val <$> bin_op_eval_compare op v1 v2) = Some v)
     (BinOp op #v1 #v2)%E v | 1.
 Proof.
-  rewrite to_val_unseal /=. apply (pure_exec_pure_wp O).
+  rewrite into_val_unseal /=. apply (pure_exec_pure_wp O).
   intros [??]. assert (bin_op_eval op (LitV v1) (LitV v2) = Some v).
   { rewrite /bin_op_eval decide_False // /=. destruct op; try by simpl in *. }
   revert H. solve_pure_exec.
@@ -294,10 +294,10 @@ Qed.
 
 Global Instance wp_w8_binop op (v1 v2 : w8) (v : val) :
   PureWp (op ≠ EqOp ∧
-      (to_val <$> bin_op_eval_word op v1 v2) ∪ (to_val <$> bin_op_eval_compare op v1 v2) = Some v)
+      (into_val <$> bin_op_eval_word op v1 v2) ∪ (into_val <$> bin_op_eval_compare op v1 v2) = Some v)
     (BinOp op #v1 #v2)%E v | 1.
 Proof.
-  rewrite to_val_unseal /=. apply (pure_exec_pure_wp O).
+  rewrite into_val_unseal /=. apply (pure_exec_pure_wp O).
   intros [??]. assert (bin_op_eval op (LitV v1) (LitV v2) = Some v).
   { rewrite /bin_op_eval decide_False // /=. destruct op; try by simpl in *. }
   revert H. solve_pure_exec.
@@ -306,7 +306,7 @@ Qed.
 Global Instance wp_w8_w64_binop op (v1 : w8) (v2 : w64) (v : w8) :
   PureWp (bin_op_eval_shift op v1 (W8 (uint.Z v2)) = Some v) (BinOp op #v1 #v2) #v | 1.
 Proof.
-  rewrite to_val_unseal. apply (pure_exec_pure_wp O).
+  rewrite into_val_unseal. apply (pure_exec_pure_wp O).
   rewrite /bin_op_eval_shift /=.
   intros H. destruct op; simpl in H; try by exfalso.
   all: revert H; solve_pure_exec; inversion H; subst; done.
@@ -315,7 +315,7 @@ Qed.
 Global Instance wp_w8_w16_binop op (v1 : w8) (v2 : w16) (v : w8) :
   PureWp (bin_op_eval_shift op v1 (W8 (uint.Z v2)) = Some v) (BinOp op #v1 #v2) #v | 1.
 Proof.
-  rewrite to_val_unseal. apply (pure_exec_pure_wp O).
+  rewrite into_val_unseal. apply (pure_exec_pure_wp O).
   intros H. destruct op; simpl in H; try by exfalso.
   all: revert H; solve_pure_exec; inversion H; subst; done.
 Qed.
@@ -323,7 +323,7 @@ Qed.
 Global Instance wp_w8_w32_binop op (v1 : w8) (v2 : w32) (v : w8) :
   PureWp (bin_op_eval_shift op v1 (W8 (uint.Z v2)) = Some v) (BinOp op #v1 #v2) #v | 1.
 Proof.
-  rewrite to_val_unseal. apply (pure_exec_pure_wp O).
+  rewrite into_val_unseal. apply (pure_exec_pure_wp O).
   intros H. destruct op; simpl in H; try by exfalso.
   all: revert H; solve_pure_exec; inversion H; subst; done.
 Qed.
@@ -331,7 +331,7 @@ Qed.
 Global Instance wp_w32_w64_binop op (v1 : w32) (v2 : w64) (v : w32) :
   PureWp (bin_op_eval_shift op v1 (W32 (uint.Z v2)) = Some v) (BinOp op #v1 #v2) #v | 1.
 Proof.
-  rewrite to_val_unseal. apply (pure_exec_pure_wp O).
+  rewrite into_val_unseal. apply (pure_exec_pure_wp O).
   intros H. destruct op; simpl in H; try by exfalso.
   all: revert H; solve_pure_exec; inversion H; subst; done.
 Qed.
@@ -339,7 +339,7 @@ Qed.
 Global Instance wp_w32_w16_binop op (v1 : w32) (v2 : w16) (v : w32) :
   PureWp (bin_op_eval_shift op v1 (W32 (uint.Z v2)) = Some v) (BinOp op #v1 #v2) #v | 1.
 Proof.
-  rewrite to_val_unseal. apply (pure_exec_pure_wp O).
+  rewrite into_val_unseal. apply (pure_exec_pure_wp O).
   intros H. destruct op; simpl in H; try by exfalso.
   all: revert H; solve_pure_exec; inversion H; subst; done.
 Qed.
@@ -347,7 +347,7 @@ Qed.
 Global Instance wp_w32_w8_binop op (v1 : w32) (v2 : w8) (v : w32) :
   PureWp (bin_op_eval_shift op v1 (W32 (uint.Z v2)) = Some v) (BinOp op #v1 #v2) #v | 1.
 Proof.
-  rewrite to_val_unseal. apply (pure_exec_pure_wp O).
+  rewrite into_val_unseal. apply (pure_exec_pure_wp O).
   intros H. destruct op; simpl in H; try by exfalso.
   all: revert H; solve_pure_exec; inversion H; subst; done.
 Qed.
@@ -355,7 +355,7 @@ Qed.
 Global Instance wp_w64_w16_binop op (v1 : w64) (v2 : w16) (v : w64) :
   PureWp (bin_op_eval_shift op v1 (W64 (uint.Z v2)) = Some v) (BinOp op #v1 #v2) #v | 1.
 Proof.
-  rewrite to_val_unseal. apply (pure_exec_pure_wp O).
+  rewrite into_val_unseal. apply (pure_exec_pure_wp O).
   intros H. destruct op; simpl in H; try by exfalso.
   all: revert H; solve_pure_exec; inversion H; subst; done.
 Qed.
@@ -363,7 +363,7 @@ Qed.
 Global Instance wp_w64_w8_binop op (v1 : w64) (v2 : w8) (v : w64) :
   PureWp (bin_op_eval_shift op v1 (W64 (uint.Z v2)) = Some v) (BinOp op #v1 #v2) #v | 1.
 Proof.
-  rewrite to_val_unseal. apply (pure_exec_pure_wp O).
+  rewrite into_val_unseal. apply (pure_exec_pure_wp O).
   intros H. destruct op; simpl in H; try by exfalso.
   all: revert H; solve_pure_exec; inversion H; subst; done.
 Qed.
@@ -371,7 +371,7 @@ Qed.
 Global Instance wp_w64_w32_binop op (v1 : w64) (v2 : w32) (v : w64) :
   PureWp (bin_op_eval_shift op v1 (W64 (uint.Z v2)) = Some v) (BinOp op #v1 #v2) #v | 1.
 Proof.
-  rewrite to_val_unseal. apply (pure_exec_pure_wp O).
+  rewrite into_val_unseal. apply (pure_exec_pure_wp O).
   intros H. destruct op; simpl in H; try by exfalso.
   all: revert H; solve_pure_exec; inversion H; subst; done.
 Qed.
@@ -379,7 +379,7 @@ Qed.
 Global Instance wp_w16_w64_binop op (v1 : w16) (v2 : w64) (v : w16) :
   PureWp (bin_op_eval_shift op v1 (W16 (uint.Z v2)) = Some v) (BinOp op #v1 #v2) #v | 1.
 Proof.
-  rewrite to_val_unseal. apply (pure_exec_pure_wp O).
+  rewrite into_val_unseal. apply (pure_exec_pure_wp O).
   intros H. destruct op; simpl in H; try by exfalso.
   all: revert H; solve_pure_exec; inversion H; subst; done.
 Qed.
@@ -387,7 +387,7 @@ Qed.
 Global Instance wp_w16_w32_binop op (v1 : w16) (v2 : w32) (v : w16) :
   PureWp (bin_op_eval_shift op v1 (W16 (uint.Z v2)) = Some v) (BinOp op #v1 #v2) #v | 1.
 Proof.
-  rewrite to_val_unseal. apply (pure_exec_pure_wp O).
+  rewrite into_val_unseal. apply (pure_exec_pure_wp O).
   intros H. destruct op; simpl in H; try by exfalso.
   all: revert H; solve_pure_exec; inversion H; subst; done.
 Qed.
@@ -395,7 +395,7 @@ Qed.
 Global Instance wp_w16_w8_binop op (v1 : w16) (v2 : w8) (v : w16) :
   PureWp (bin_op_eval_shift op v1 (W16 (uint.Z v2)) = Some v) (BinOp op #v1 #v2) #v | 1.
 Proof.
-  rewrite to_val_unseal. apply (pure_exec_pure_wp O).
+  rewrite into_val_unseal. apply (pure_exec_pure_wp O).
   intros H. destruct op; simpl in H; try by exfalso.
   all: revert H; solve_pure_exec; inversion H; subst; done.
 Qed.
@@ -404,7 +404,7 @@ Qed.
 Global Instance wp_bool_binop op (v1 v2 v : bool) :
   PureWp (op ≠ EqOp ∧ bin_op_eval_bool op v1 v2 = Some v) (BinOp op #v1 #v2) #v | 1.
 Proof.
-  rewrite to_val_unseal. apply (pure_exec_pure_wp O).
+  rewrite into_val_unseal. apply (pure_exec_pure_wp O).
   case => ?. solve_pure_exec.
   - rewrite /bin_op_eval decide_False // b /=. Transitions.monad_simpl.
   - rewrite /bin_op_eval decide_False // b /= in H0. by Transitions.monad_inv.
@@ -413,7 +413,7 @@ Qed.
 Global Instance wp_string_binop op (v1 v2 v : go_string) :
   PureWp (op ≠ EqOp ∧ bin_op_eval_string op v1 v2 = Some v) (BinOp op #v1 #v2) #v | 1.
 Proof.
-  rewrite to_val_unseal. apply (pure_exec_pure_wp O).
+  rewrite into_val_unseal. apply (pure_exec_pure_wp O).
   case => ?. solve_pure_exec.
   - rewrite /bin_op_eval decide_False // b /=. Transitions.monad_simpl.
   - rewrite /bin_op_eval decide_False // b /= in H0. by Transitions.monad_inv.
@@ -421,14 +421,14 @@ Qed.
 
 Global Instance wp_offset k (l : loc) (off : w64) :
   PureWp True (BinOp (OffsetOp k) #l #off) #(l +ₗ k * (uint.Z off)).
-Proof. rewrite to_val_unseal. apply (pure_exec_pure_wp O). solve_pure_exec. Qed.
+Proof. rewrite into_val_unseal. apply (pure_exec_pure_wp O). solve_pure_exec. Qed.
 
 (* string lookup ops *)
 
 Global Instance wp_StringGet_w64 (s : go_string) (i : w64) (v : w8) :
   PureWp (s !! uint.nat i = Some v) (StringGet #s #i) #v.
 Proof.
-  rewrite to_val_unseal. apply (pure_exec_pure_wp O). solve_pure_exec.
+  rewrite into_val_unseal. apply (pure_exec_pure_wp O). solve_pure_exec.
   - rewrite /bin_op_eval /= H /=. Transitions.monad_simpl.
   - rewrite /bin_op_eval /= H /= in H1. Transitions.monad_inv. done.
 Qed.
@@ -436,7 +436,7 @@ Qed.
 Global Instance wp_StringGet_w32 (s : go_string) (i : w32) (v : w8) :
   PureWp (s !! uint.nat i = Some v) (StringGet #s #i) #v.
 Proof.
-  rewrite to_val_unseal. apply (pure_exec_pure_wp O). solve_pure_exec.
+  rewrite into_val_unseal. apply (pure_exec_pure_wp O). solve_pure_exec.
   - rewrite /bin_op_eval /= H /=. Transitions.monad_simpl.
   - rewrite /bin_op_eval /= H /= in H1. Transitions.monad_inv. done.
 Qed.
@@ -444,7 +444,7 @@ Qed.
 Global Instance wp_StringGet_w16 (s : go_string) (i : w16) (v : w8) :
   PureWp (s !! uint.nat i = Some v) (StringGet #s #i) #v.
 Proof.
-  rewrite to_val_unseal. apply (pure_exec_pure_wp O). solve_pure_exec.
+  rewrite into_val_unseal. apply (pure_exec_pure_wp O). solve_pure_exec.
   - rewrite /bin_op_eval /= H /=. Transitions.monad_simpl.
   - rewrite /bin_op_eval /= H /= in H1. Transitions.monad_inv. done.
 Qed.
@@ -452,7 +452,7 @@ Qed.
 Global Instance wp_StringGet_w8 (s : go_string) (i : w8) (v : w8) :
   PureWp (s !! uint.nat i = Some v) (StringGet #s #i) #v.
 Proof.
-  rewrite to_val_unseal. apply (pure_exec_pure_wp O). solve_pure_exec.
+  rewrite into_val_unseal. apply (pure_exec_pure_wp O). solve_pure_exec.
   - rewrite /bin_op_eval /= H /=. Transitions.monad_simpl.
   - rewrite /bin_op_eval /= H /= in H1. Transitions.monad_inv. done.
 Qed.
@@ -467,7 +467,7 @@ Proof. apply (pure_exec_pure_wp O). solve_pure_exec. Qed.
 
 Global Instance wp_call_go_func (v2 : val) f x e :
   PureWp True (App #(func.mk f x e) v2) (subst' x v2 (subst' f #(func.mk f x e) e)).
-Proof. rewrite to_val_unseal /=. apply (pure_exec_pure_wp O). solve_pure_exec. Qed.
+Proof. rewrite into_val_unseal /=. apply (pure_exec_pure_wp O). solve_pure_exec. Qed.
 
 End instances.
 
@@ -700,52 +700,35 @@ Tactic Notation "wp_apply" open_constr(lem) :=
 
 (* FIXME: rest of the instances *)
 Section go_wp_pure_instances.
-Context `{ffi_sem: ffi_semantics} `{!ffi_interp ffi} `{!gooseGlobalGS Σ, !gooseLocalGS Σ}
-         `{!GoContext}.
-Context `{goose_go_stepper = go.is_go_step}.
+Context `{ffi_sem: ffi_semantics} `{!ffi_interp ffi} `{!gooseGlobalGS Σ, !gooseLocalGS Σ}.
 
+Local Ltac solve_pure :=
+  iIntros "% * _ % HΦ"; iApply wp_GoInstruction;
+  [ intros; repeat econstructor | ];
+  iNext; iIntros "* %Hstep"; inv Hstep; inv Hpure;
+  iFrame; by iIntros "$".
 Global Instance wp_GoAlloc t :
   PureWp True (GoInstruction (GoAlloc t) #()) (alloc t #()).
-Proof.
-  iIntros "% * _ % HΦ". iApply wp_GoInstruction; rewrite H0.
-  { intros. repeat econstructor. }
-  iNext. iIntros "* %Hstep". inv Hstep. inv Hpure.
-  iFrame. by iIntros "$".
-Qed.
+Proof. solve_pure. Qed.
 
 Global Instance wp_GoStore t (l : loc) v :
   PureWp True (GoInstruction (GoStore t) (#l, v)%V) (store t #l v).
-Proof.
-  iIntros "% * _ % HΦ". rewrite to_val_unseal. iApply wp_GoStore. iApply "HΦ".
-Qed.
+Proof. solve_pure. Qed.
 
 Global Instance wp_GoLoad t (l : loc) :
   PureWp True (GoInstruction (GoLoad t) #l) (load t #l).
-Proof.
-  iIntros "% * _ % HΦ". rewrite to_val_unseal. iApply wp_GoLoad. iApply "HΦ".
-Qed.
-
-(* TODO: would be ok to make functions and method total functions. The go
-   compiler will make sure that only valid functions get called. To deal with
-   method sets, we'll anyways want a different piece of state that has all of
-   the method signatures for a type, so it's OK for the methods map to have
-   method implementations for every method name (the ones that don't exist will
-   never be called). *)
+Proof. solve_pure. Qed.
 
 Global Instance wp_GlobalVarAddr v :
   PureWp True (GoInstruction (GlobalVarAddr v) #()) #(global_addr v).
-Proof.
-  iIntros "% * _ % HΦ". rewrite to_val_unseal. wp_apply wp_GlobalVarAddr. iApply "HΦ".
-Qed.
+Proof. solve_pure. Qed.
 
 Global Instance wp_StructFieldRef t f (l : loc) :
   PureWp True (GoInstruction (StructFieldRef t f) #l) #(struct_field_ref t f l).
-Proof.
-  iIntros "% * _ % HΦ". rewrite to_val_unseal. wp_apply wp_StructFieldRef. iApply "HΦ".
-Qed.
+Proof. solve_pure. Qed.
 
 Global Instance wp_StructFieldSet_untyped f m v :
   PureWp True (GoInstruction (StructFieldSet f) (StructV m, v)%V) (StructV (<[f := v]> m)).
-Proof. iIntros "% * _ % HΦ". wp_apply wp_StructFieldSet. iApply "HΦ". Qed.
+Proof. solve_pure. Qed.
 
 End go_wp_pure_instances.
